$$
\frac{d_{ia}}{dt}=\frac{1}{L_a}(-R_ai_a-e_s  +vin)\space(1)
\\\frac{d_{ia}}{dt}=\frac{1}{L_a}(-R_ai_a-k_\omega \omega +vin)\space (2)
\\\frac{\omega(s)}{vin(s)}=\frac{k_m}{LJs^2+s(RJ+LB)+RB+k_mk_a}\space (3)
\\\omega_2=\frac{\omega_1 R1}{R2}\space (4)
\\\frac{\omega 2(s)}{\omega_1 (s)}=\frac{R1}{R2}\space (5)
\\ v_1=\frac{p\omega_2}{60}\space (6)
\\\frac{v_1(s)}{\omega_2(s)}=\frac{p}{60}\space (7)
\\\frac{\omega_1(s)}{vin(s)}*\frac{\omega 2(s)}{\omega_1 (s)}*\frac{v_1(s)}{\omega_2(s)}=\frac{v1(s)}{vin(s)}=\frac{x1(s)}{s*vin(s)}\space(8)
\\G(s)=\frac{k_mR_1P}{R_260LJs^3+R_260s^2(RJ+LB)+(RB+k_mk_a)R_260s}\space (9)
\\G(c)=\frac{kd2s^4+kds^3+kps^2+kis+ki2}{s^2}\space (10)
\\ \frac{G(s)G(c)}{1+G(s)G(c)}=\frac{(0.5*kd2*s^4 + 0.5*kd*s^3 + 0.5*kp*s^2 + 0.5*ki*s + 0.5*ki2)}{(s^5 + (0.5*kd2 + 2.0)*s^4 + (0.5*kd + 2.0)*s^3 + 0.5*kp*s^2 + 0.5*ki*s + 0.5*ki2)}
\\Pd=\frac{\omega^2}{(s^2+2\zeta\omega+\omega^2)(s+\beta2\zeta\omega)^3}\space (11)
\\DenPd=s^5 + 8.53*s^4 + 25.7*s^3 + 31.0*s^2 + 11.8*s + 1.49\space (12)
$$

